FreydSSA/Body.lean
@@ -1,0 +1,277 @@
+import Mathlib.Data.List.Basic
+import Std.Data.List.Basic
+import Mathlib.Data.Set.Basic
+import Mathlib.Data.Set.Function
+import Mathlib.Init.Classical
+
+import FreydSSA.Ctx
+import FreydSSA.InstSet
+import FreydSSA.Tm
+
+inductive InstSet.Body {ν : Type u} {α : Type v} (Φ : InstSet (Ty α))
+  : Purity → Ctx ν (Ty α) → Ctx ν (Ty α) → Type (max u v) where
+  | nil (p) : Γ.Wk Δ → Body Φ p Γ Δ
+  | let1 : Φ.Tm p Γ a → Body Φ p (⟨x, a⟩::Γ) Δ → Body Φ p Γ Δ
+  | let2 : Φ.Tm p Γ (Ty.pair A B)
+    → Body Φ p (⟨x, A⟩::⟨y, B⟩::Γ) Δ
+    → Body Φ p Γ Δ
+
+inductive InstSet.Body.Iso {Φ : InstSet (Ty α)}: Φ.Body p Γ Δ → Φ.Body p Γ' Δ' → Prop
+  | nil (p) : w.Iso w' → Iso (Body.nil p w) (Body.nil p w')
+  | let1 : Tm.Iso e e' → Body.Iso b b' → Iso (Body.let1 e b) (Body.let1 e' b')
+  | let2 : Tm.Iso e e' → Body.Iso b b' → Iso (Body.let2 e b) (Body.let2 e' b')
+
+theorem InstSet.Body.Iso.refl {Φ : InstSet (Ty α)} {Γ Δ : Ctx ν (Ty α)} {p}
+  (e : Φ.Body p Γ Δ)
+  : e.Iso e
+  := by induction e with
+  | nil _ I => constructor; exact I.iso_refl
+  | _ =>
+    constructor
+    . apply Tm.Iso.refl
+    . apply_assumption
+
+theorem InstSet.Body.Iso.symm {Φ : InstSet (Ty α)}
+  {e : Φ.Body p Γ Δ} {e' : Φ.Body p Γ' Δ'}
+  (h : e.Iso e') : e'.Iso e
+  := by induction h with
+  | nil _ I => constructor; exact I.symm
+  | _ =>
+    constructor
+    . apply Tm.Iso.symm; assumption
+    . apply_assumption
+
+theorem InstSet.Body.Iso.trans {Φ : InstSet (Ty α)}
+  {e : Φ.Body p Γ Δ} {e' : Φ.Body p Γ' Δ'} {e'' : Φ.Body p Γ'' Δ''}
+  (h : e.Iso e') (h' : e'.Iso e'') : e.Iso e''
+  := by induction h generalizing Γ'' Δ'' with
+  | nil _ I => cases h'; constructor; apply I.trans; assumption
+  | _ =>
+    cases h'
+    constructor
+    . apply Tm.Iso.trans <;> assumption
+    . apply_assumption; assumption
+
+def InstSet.Body.to_impure {Φ : InstSet (Ty α)} {Γ Δ : Ctx ν (Ty α)}
+  : Φ.Body p Γ Δ → Φ.Body 0 Γ Δ
+  | nil _ h => nil 0 h
+  | let1 e b => let1 e.to_impure b.to_impure
+  | let2 e b => let2 e.to_impure b.to_impure
+
+def InstSet.Body.wk_entry {Φ : InstSet (Ty α)} {Γ Δ Ξ : Ctx ν (Ty α)}
+  : Γ.Wk Δ → Φ.Body p Δ Ξ → Φ.Body p Γ Ξ
+  | h, nil p h' => nil p (h.comp h')
+  | h, let1 e b => let1 (Tm.wk h e) (wk_entry (h.cons _) b)
+  | h, let2 e b => let2 (Tm.wk h e) (wk_entry ((h.cons _).cons _) b)
+
+def InstSet.Body.wk_exit {Φ : InstSet (Ty α)} {Γ Δ Ξ : Ctx ν (Ty α)}
+  : Φ.Body p Γ Δ → Δ.Wk Ξ → Φ.Body p Γ Ξ
+  | nil p h, h' => nil p (h.comp h')
+  | let1 e b, h' => let1 e (wk_exit b h')
+  | let2 e b, h' => let2 e (wk_exit b h')
+
+def InstSet.Body.comp {Φ : InstSet (Ty α)} {Γ Δ Ξ : Ctx ν (Ty α)}
+  : Φ.Body p Γ Δ → Φ.Body p Δ Ξ → Φ.Body p Γ Ξ
+  | nil p h, b => wk_entry h b
+  | let1 e b, b' => let1 e (comp b b')
+  | let2 e b, b' => let2 e (comp b b')
+
+theorem InstSet.Body.Iso.wk_entry {Φ : InstSet (Ty α)}
+  {Γ Δ Ξ : Ctx ν (Ty α)} {Γ' Δ' Ξ' : Ctx ν' (Ty α)}
+  {w: Γ.Wk Δ} {w': Γ'.Wk Δ'} {b: Φ.Body p Δ Ξ} {b': Φ.Body p Δ' Ξ'}
+  (hw: w.Iso w') (hb: b.Iso b')
+  : (wk_entry w b).Iso (wk_entry w' b')
+  := by induction hb with
+  | nil => simp only [Body.wk_entry]; constructor; apply Ctx.Wk.Iso.comp <;> assumption
+  | _ =>
+    simp only [Body.wk_entry]
+    constructor
+    . apply Tm.Iso.wk <;> assumption
+    . apply_assumption
+      repeat constructor
+      assumption
+
+theorem InstSet.Body.Iso.wk_exit {Φ : InstSet (Ty α)}
+  {Γ Δ Ξ' : Ctx ν (Ty α)} {Γ' Δ' Ξ' : Ctx ν' (Ty α)}
+  {b: Φ.Body p Γ Δ} {b': Φ.Body p Γ' Δ'} {w: Δ.Wk Ξ} {w': Δ'.Wk Ξ'}
+  (hw: w.Iso w') (hb: b.Iso b')
+  : (wk_exit b w).Iso (wk_exit b' w')
+  := by induction hb with
+  | nil => simp only [Body.wk_exit]; constructor; apply Ctx.Wk.Iso.comp <;> assumption
+  | _ =>
+    simp only [Body.wk_exit]
+    constructor
+    . assumption
+    . apply_assumption <;> assumption
+
+theorem InstSet.Body.Iso.comp {Φ: InstSet (Ty α)}
+  {l: Φ.Body p Γ Δ} {l': Φ.Body p Γ' Δ'}
+  {r: Φ.Body p Δ Ξ} {r': Φ.Body p Δ' Ξ'}
+  (hl: l.Iso l') (hr: r.Iso r')
+  : (l.comp r).Iso (l'.comp r')
+  := by induction hl with
+  | nil _ hw => simp only [Body.comp]; exact wk_entry hw hr
+  | _ =>
+    simp only [Body.comp]
+    constructor
+    . assumption
+    . apply_assumption; assumption
+
+inductive InstSet.Body.InjOn {Φ : InstSet (Ty α)} (ρ : ν → ν')
+  : {Γ Δ: Ctx ν (Ty α)} → Φ.Body p Γ Δ → Prop
+  | nil {Γ Δ: Ctx ν (Ty α)} (h: Γ.Wk Δ): Γ.InjOn ρ → Body.InjOn ρ (Body.nil p h)
+  | let1 {b: Φ.Body p (⟨x, A⟩::Γ) Δ} (e: Φ.Tm p Γ A): b.InjOn ρ → (b.let1 e).InjOn ρ
+  | let2 {b: Φ.Body p (⟨x, A⟩::⟨y, B⟩::Γ) Δ} (e: Φ.Tm p Γ (Ty.pair A B)):
+    b.InjOn ρ → (b.let2 e).InjOn ρ
+
+def InstSet.Body.InjOn.entry {Φ : InstSet (Ty α)} {Γ Δ : Ctx ν (Ty α)} {p}
+  {b : Φ.Body p Γ Δ} {ρ : ν → ν'} : b.InjOn ρ → Γ.InjOn ρ
+  | nil _ h => h
+  | let1 _ h => h.entry.tail
+  | let2 _ h => h.entry.tail.tail
+
+def InstSet.Body.InjOn.exit {Φ : InstSet (Ty α)} {Γ Δ : Ctx ν (Ty α)} {p}
+  {b : Φ.Body p Γ Δ} {ρ : ν → ν'} : b.InjOn ρ → Δ.InjOn ρ
+  | nil w h => h.wk w
+  | let1 _ h => h.exit
+  | let2 _ h => h.exit
+
+inductive InstSet.Body.Fresh {Φ : InstSet (Ty α)} (n: ν)
+  : {Γ Δ: Ctx ν (Ty α)} → Φ.Body p Γ Δ → Prop
+  | nil {Γ Δ: Ctx ν (Ty α)} (h: Γ.Wk Δ): Γ.Fresh n → Body.Fresh n (Body.nil p h)
+  | let1 {b: Φ.Body p (⟨x, A⟩::Γ) Δ} (e: Φ.Tm p Γ A): b.Fresh n → (b.let1 e).Fresh n
+  | let2 {b: Φ.Body p (⟨x, A⟩::⟨y, B⟩::Γ) Δ} (e: Φ.Tm p Γ (Ty.pair A B)):
+    b.Fresh n → (b.let2 e).Fresh n
+
+theorem InstSet.Body.Fresh.entry {Φ : InstSet (Ty α)} {Γ Δ : Ctx ν (Ty α)} {p}
+  {b : Φ.Body p Γ Δ} {n} : b.Fresh n → Γ.Fresh n
+  | nil _ h => h
+  | let1 _ h => h.entry.tail
+  | let2 _ h => h.entry.tail.tail
+
+theorem InstSet.Body.Fresh.exit {Φ : InstSet (Ty α)} {Γ Δ : Ctx ν (Ty α)} {p}
+  {b : Φ.Body p Γ Δ} {n} : b.Fresh n → Δ.Fresh n
+  | nil w h => h.wk w
+  | let1 _ h => h.exit
+  | let2 _ h => h.exit
+
+def InstSet.Body.defs {Φ : InstSet (Ty α)} {Γ Δ : Ctx ν (Ty α)}
+  : Φ.Body p Γ Δ → List ν
+  | nil _ _ => []
+  | @let1 _ _ _ _ _ _ x _ _ b => x::b.defs
+  | @let2 _ _ _ _ _ _ _ x y _ _ b => x::y::b.defs
+
+inductive InstSet.Body.NotDef {Φ : InstSet (Ty α)} (n: ν)
+  : {Γ Δ : Ctx ν (Ty α)} → Φ.Body p Γ Δ → Prop
+  | nil {Γ Δ: Ctx ν (Ty α)} (h: Γ.Wk Δ): Body.NotDef n (Body.nil p h)
+  | let1 {b: Φ.Body p (⟨x, A⟩::Γ) Δ}: x ≠ n → (e: Φ.Tm p Γ A) →
+    b.NotDef n → (b.let1 e).NotDef n
+  | let2 {b: Φ.Body p (⟨x, A⟩::⟨y, B⟩::Γ) Δ}: x ≠ n → y ≠ n →
+    (e: Φ.Tm p Γ (Ty.pair A B)) → b.NotDef n → (b.let2 e).NotDef n
+
+theorem InstSet.Body.NotDef.not_mem_defs {Φ: InstSet (Ty α)} {b: Φ.Body p Γ Δ}
+  : b.NotDef n → n ∉ b.defs
+  | nil _ => by simp [defs]
+  | let1 hx e b => by
+    simp only [defs, List.mem_cons, not_or]
+    exact ⟨hx.symm, b.not_mem_defs⟩
+  | let2 hx hy e b => by
+    simp only [defs, List.mem_cons, not_or]
+    exact ⟨hx.symm, hy.symm, b.not_mem_defs⟩
+
+theorem InstSet.Body.NotDef.of_not_mem_defs {Φ: InstSet (Ty α)} {b: Φ.Body p Γ Δ}
+  : n ∉ b.defs → b.NotDef n
+  := by induction b with
+  | nil => exact λ_ => NotDef.nil _
+  | let1 _ _ I =>
+    simp only [defs, List.mem_cons, not_or, and_imp]
+    intro hx hn
+    constructor
+    exact Ne.symm hx
+    exact I hn
+  | let2 _ _ I =>
+    simp only [defs, List.mem_cons, not_or, and_imp]
+    intro hx hy hn
+    constructor
+    exact Ne.symm hx
+    exact Ne.symm hy
+    exact I hn
+
+theorem InstSet.Body.NotDef.iff_not_mem_defs {Φ: InstSet (Ty α)} {b: Φ.Body p Γ Δ}
+  : b.NotDef n ↔ n ∉ b.defs
+  := ⟨not_mem_defs, of_not_mem_defs⟩
+
+theorem InstSet.Body.Fresh.notDef {Φ : InstSet (Ty α)} {Γ Δ : Ctx ν (Ty α)} {p}
+  {b : Φ.Body p Γ Δ} {n} : b.Fresh n → b.NotDef n
+  | nil _ h => NotDef.nil _
+  | let1 _ h => NotDef.let1 h.entry.head _ h.notDef
+  | let2 _ h => NotDef.let2 h.entry.head h.entry.tail.head _ h.notDef
+
+theorem InstSet.Body.NotDef.toFresh {Φ: InstSet (Ty α)} {Γ Δ : Ctx ν (Ty α)} {p}
+  {b: Φ.Body p Γ Δ} {n} (hb: b.NotDef n) (hΓ: Γ.Fresh n): b.Fresh n
+  := by induction hb with
+  | _ =>
+    constructor
+    apply_assumption
+    repeat first | apply Ctx.Fresh.cons | assumption
+
+inductive InstSet.Body.SSA {Φ: InstSet (Ty α)}
+  : {Γ Δ: Ctx ν (Ty α)} → Φ.Body p Γ Δ → Prop
+  | nil {Γ Δ: Ctx ν (Ty α)} (h: Γ.Wk Δ): Body.SSA (Body.nil p h)
+  | let1 {b: Φ.Body p (⟨x, A⟩::Γ) Δ}:
+    Ctx.Fresh x Γ → (e: Φ.Tm p Γ A) → b.SSA → (b.let1 e).SSA
+  | let2 {b: Φ.Body p (⟨x, A⟩::⟨y, B⟩::Γ) Δ}:
+      x ≠ y →
+      Ctx.Fresh x Γ →
+      Ctx.Fresh y Γ →
+      (e: Φ.Tm p Γ (Ty.pair A B)) →
+      b.SSA →
+      (b.let2 e).SSA
+
+def InstSet.Body.αSSA {Φ: InstSet (Ty α)} (b: Φ.Body p Γ Δ): Prop
+  := ∃b' : Φ.Body p Γ Δ, b'.SSA ∧ b.Iso b'
+
+structure InstSet.Body.Renaming {Φ: InstSet (Ty α)}
+  {Γ Δ : Ctx ν (Ty α)} (b: Φ.Body p Γ Δ) (Γ' Δ': Ctx ν' (Ty α))
+  where
+  val : Φ.Body p Γ' Δ'
+  isIso : b.Iso val
+
+structure InstSet.Body.SSAForm {Φ: InstSet (Ty α)}
+  {Γ Δ : Ctx ν (Ty α)} (b: Φ.Body p Γ Δ) (Γ' Δ': Ctx ν' (Ty α))
+  extends Renaming b Γ' Δ' where
+  isSSA : val.SSA
+
+structure InstSet.SSABody {Φ: InstSet (Ty α)} (p: Purity) (Γ Δ: Ctx ν (Ty α)) where
+  val : Φ.Body p Γ Δ
+  isSSA : val.SSA
+
+-- TODO: every body, w/ de-Bruijn indices, can be placed into SSA...
+
+-- TODO: in particular, if ν is infinite (or actually, just > |b| + |Γ|), then every body from Γ to
+--Δ is in αSSA
+
+--TODO: InstSet.InjOn case helpers?
+def InstSet.Body.rename {Φ : InstSet (Ty α)} {Γ Δ : Ctx ν (Ty α)}
+  {ρ : ν → ν'} : {b : Φ.Body p Γ Δ} → b.InjOn ρ → Φ.Body p (Γ.rename ρ) (Δ.rename ρ)
+  | nil _ h, hρ => nil _ (h.rename (by cases hρ; assumption))
+  | let1 e b, hρ => let1 (e.rename hρ.entry) (b.rename (by cases hρ; assumption))
+  | let2 e b, hρ => let2 (e.rename hρ.entry) (b.rename (by cases hρ; assumption))
+
+theorem InstSet.Body.rename_iso {Φ : InstSet (Ty α)} {Γ Δ : Ctx ν (Ty α)}
+  {ρ : ν → ν'} {b : Φ.Body p Γ Δ} (hb: b.InjOn ρ): b.Iso (b.rename hb)
+  := by induction b with
+  | nil _ h =>
+    simp only [rename]
+    constructor
+    exact h.rename_iso (hb.entry)
+  | let1 e b I =>
+    simp only [rename]
+    constructor
+    exact e.rename_iso (hb.entry)
+    apply I
+  | let2 e b I =>
+    simp only [rename]
+    constructor
+    exact e.rename_iso (hb.entry)
+    apply I
