FreydSSA/InstSet.lean
@@ -1,0 +1,25 @@
+inductive Ty (α: Type u): Type u where
+  | base (a : α)
+  | pair (a b : Ty α)
+  | unit
+  | bool
+
+inductive Purity
+  | pure
+  | impure
+
+instance : OfNat Purity 0 where
+  ofNat := Purity.impure
+
+instance : OfNat Purity 1 where
+  ofNat := Purity.pure
+
+structure InstSet (α : Type u) : Type _ where
+  Op : Purity → α → α → Type
+  pure_to_impure : Op 1 a b → Op 0 a b
+
+def InstSet.to_impure {α : Type u} (Φ : InstSet α) {p} {A B : α} (f : Φ.Op p A B)
+  : Φ.Op 0 A B
+  := match p with
+  | Purity.pure => Φ.pure_to_impure f
+  | Purity.impure => f
