FreydSSA/Tm.lean
@@ -1,0 +1,88 @@
+import Mathlib.Data.List.Basic
+import Std.Data.List.Basic
+import Mathlib.Data.Set.Basic
+import Mathlib.Data.Set.Function
+import Mathlib.Init.Classical
+
+import FreydSSA.Ctx
+import FreydSSA.InstSet
+
+inductive InstSet.Tm {ν : Type u} {α : Type v} (Φ : InstSet (Ty α))
+  : Purity → Ctx ν (Ty α) → Ty α → Type (max u v) where
+  | var {n a} (p) : Γ.Wk [⟨n, a⟩] → Tm Φ p Γ a
+  | op (f: Φ.Op p A B) : Tm Φ 1 Γ A → Tm Φ p Γ B
+  | pair (p) : Tm Φ 1 Γ A → Tm Φ 1 Γ B → Tm Φ p Γ (Ty.pair A B)
+  | unit (p) : Tm Φ p Γ Ty.unit
+  | bool (p) (b: Bool) : Tm Φ p Γ Ty.bool
+
+inductive InstSet.Tm.IsoSh {Φ : InstSet (Ty α)}: Φ.Tm p Γ A → Φ.Tm p' Γ' A' → Prop
+  | var (p p') : w.Iso w' → IsoSh (Tm.var p w) (Tm.var p' w')
+  | op (f) : Tm.IsoSh e e' → IsoSh (Tm.op f e) (Tm.op f e')
+  | pair (p p') : Tm.IsoSh l l' → Tm.IsoSh r r' → IsoSh (Tm.pair p l r) (Tm.pair p' l' r')
+  | unit (p p') : IsoSh (Tm.unit p) (Tm.unit p')
+  | bool (p p') : IsoSh (Tm.bool p b) (Tm.bool p' b)
+
+inductive InstSet.Tm.Iso {Φ : InstSet (Ty α)}: Φ.Tm p Γ A → Φ.Tm p Γ' A → Prop
+  | var {Γ: Ctx ν (Ty α)} {Γ': Ctx ν' (Ty α)} (p)
+    {w: Γ.Wk [⟨n, a⟩]} {w': Γ'.Wk [⟨n', a⟩]}: w.Iso w' → Iso (Tm.var p w) (Tm.var p w')
+  | op (f) : Tm.Iso e e' → Iso (Tm.op f e) (Tm.op f e')
+  | pair (p) : Tm.Iso l l' → Tm.Iso r r' → Iso (Tm.pair p l r) (Tm.pair p l' r')
+  | unit (p) : Iso (Tm.unit p) (Tm.unit p)
+  | bool (p) : Iso (Tm.bool p b) (Tm.bool p b)
+
+theorem InstSet.Tm.Iso.refl {Φ : InstSet (Ty α)} {Γ : Ctx ν (Ty α)} {A : Ty α} {e : Φ.Tm p Γ A}
+  : e.Iso e
+  := by induction e with
+  | var => constructor; apply Ctx.Wk.Iso.refl
+  | _ => constructor <;> apply_assumption
+
+theorem InstSet.Tm.Iso.symm {Φ : InstSet (Ty α)}
+  {e : Φ.Tm p Γ A} {e' : Φ.Tm p Γ' A}
+  (h : e.Iso e') : e'.Iso e
+  := by induction h with
+  | var _ I => constructor; exact I.symm
+  | _ => constructor <;> apply_assumption
+
+theorem InstSet.Tm.Iso.trans {Φ : InstSet (Ty α)}
+  {e : Φ.Tm p Γ A} {e' : Φ.Tm p Γ' A} {e'' : Φ.Tm p Γ'' A}
+  (h : e.Iso e') (h' : e'.Iso e'') : e.Iso e''
+  := by induction h with
+  | var _ I => cases h'; constructor; apply I.trans; assumption
+  | _ => cases h'; constructor <;> apply_assumption <;> assumption
+
+def InstSet.Tm.to_impure {Φ : InstSet (Ty α)} {A : Ty α} : Φ.Tm p Γ A → Φ.Tm 0 Γ A
+  | var p h => var 0 h
+  | op f e => op (Φ.to_impure f) e
+  | pair p x y => pair 0 x y
+  | unit p => unit 0
+  | bool p b => bool 0 b
+
+def InstSet.Tm.wk {Φ : InstSet (Ty α)} {A : Ty α} : Γ.Wk Δ → Φ.Tm p Δ A → Φ.Tm p Γ A
+  | h, var p h' => var p (h.comp h')
+  | h, op f e => op f (wk h e)
+  | h, pair p x y => pair p (wk h x) (wk h y)
+  | h, unit p => unit p
+  | h, bool p b => bool p b
+
+theorem InstSet.Tm.Iso.wk {Φ : InstSet (Ty α)}
+  {Γ Δ : Ctx ν (Ty α)} {Γ' Δ' : Ctx ν' (Ty α)}
+  {w : Γ.Wk Δ} {w' : Γ'.Wk Δ'}
+  {e : Φ.Tm p Δ A} {e' : Φ.Tm p Δ' A}
+  (hw : w.Iso w') (he : e.Iso e') : (e.wk w).Iso (e'.wk w')
+  := by induction he with
+  | var => simp only [Tm.wk]; constructor; apply Ctx.Wk.Iso.comp <;> assumption
+  | _ => simp only [Tm.wk]; constructor <;> apply_assumption <;> assumption
+
+def InstSet.Tm.rename {Φ : InstSet (Ty α)} {Γ : Ctx ν (Ty α)} {a : Ty α}
+  {ρ : ν → ν'} (hρ : Γ.InjOn ρ) : Φ.Tm p Γ a → Φ.Tm p (Γ.rename ρ) a
+  | var p h' => @var _ _ _ _ (ρ _) _ p (h'.rename hρ)
+  | op f e => op f (e.rename hρ)
+  | pair p l r => pair p (l.rename hρ) (r.rename hρ)
+  | unit p => unit p
+  | bool p b => bool p b
+
+theorem InstSet.Tm.rename_iso {Φ : InstSet (Ty α)} {Γ : Ctx ν (Ty α)} {a : Ty α}
+  {ρ : ν → ν'} (hρ : Γ.InjOn ρ) (e: Φ.Tm p Γ a) : e.Iso (e.rename hρ)
+  := by induction e with
+  | @var Γ n a p w => simp only [rename]; constructor; exact w.rename_iso hρ
+  | _ => simp only [rename]; constructor <;> apply_assumption
